progs/verif_printf.v
@@ -4,22 +4,54 @@ Instance CompSpecs : compspecs. make_compspecs prog. Defined.
 Definition Vprog : varspecs. mk_varspecs prog. Defined.
 
 Require Import VST.floyd.printf.
+Require Import VST.floyd.io_events.
+Require Import ITree.ITree.
+Require Import ITree.Eq.Eq.
+(*Import ITreeNotations.*)
+Notation "t1 ;; t2" := (ITree.bind t1 (fun _ => t2))
+  (at level 100, right associativity) : itree_scope.
+
+Instance nat_id : FileId := { file_id := nat; FILEid := ___sFILE; get_file_id f := O; stdout := tt }.
+
+Definition stdout := O.
 
 Definition main_spec :=
  DECLARE _main
   WITH gv : globals
-  PRE  [] main_pre prog nil gv
+  PRE  [] main_pre_ext prog (write_list stdout (string2bytes "Hello, world!
+");; write_list stdout (string2bytes "This is line 2.
+")) nil gv
   POST [ tint ] main_post prog nil gv.
 
 Definition Gprog : funspecs :=  
    ltac:(with_library prog (ltac:(make_printf_specs prog) ++ [ main_spec ])).
+
+Lemma bind_ret' : forall E (s : itree E unit), eutt eq (s;; Ret tt) s.
+Proof.
+  intros.
+  etransitivity; [|apply eq_sub_eutt, bind_ret2].
+  apply eqit_bind; [intros []|]; reflexivity.
+Qed.
 
 Lemma body_main: semax_body Vprog Gprog f_main main_spec.
 Proof.
 start_function.
 repeat do_string2bytes.
 repeat (sep_apply data_at_to_cstring; []).
-forward_printf tt.
-forward_fprintf (gv __stdout) ((Ers, string2bytes "line", gv ___stringlit_2), (Int.repr 2, tt)).
+replace_SEP 3 (ITREE (write_list stdout (string2bytes "Hello, world!
+");; write_list stdout (string2bytes "This is line 2.
+"))).
+{ go_lower; apply has_ext_ITREE. }
+forward_printf tt (write_list stdout (string2bytes "This is line 2.
+")).
+{ rewrite sepcon_comm; apply sepcon_derives; cancel.
+  apply derives_refl. }
+forward_fprintf (gv __stdout) ((Ers, string2bytes "line", gv ___stringlit_2), (Int.repr 2, tt)) (tt, Ret tt : @IO_itree file_id).
+{ (* need to know that stdout actually points to a file object? or should that be a dummy? *)
+  rewrite <- emp_sepcon at 1.
+  rewrite !sepcon_assoc; apply sepcon_derives; [admit|].
+  rewrite sepcon_comm; apply sepcon_derives; cancel.
+  apply ITREE_impl.
+  rewrite bind_ret'; reflexivity. }
 forward.
-Qed.
+Admitted.
